-

Qrl.v
@@ -10,6 +10,8 @@ Import Q.Notations.
 Definition phony_Q_sub (a b : Q) := a.
 Definition phony_Q_div (a b : Q) := a.
 
+Definition Q_inversible (a : Q) := a ≠ 0%Q.
+
 Canonical Structure Q_ring_like_op : ring_like_op Q :=
   {| rngl_has_opp := true;
      rngl_has_inv := true;
@@ -21,6 +23,7 @@ Canonical Structure Q_ring_like_op : ring_like_op Q :=
      rngl_opp := Q.opp;
      rngl_inv := Q.inv;
      rngl_le := Q.le;
+     rngl_inversible := Q_inversible;
      rngl_opt_sub := phony_Q_sub;
      rngl_opt_div := phony_Q_div |}.
 
@@ -72,6 +75,20 @@ apply Heab.
 now apply Q.le_antisymm; apply Q.lt_le_incl.
 Qed.
 
+Theorem Q_inversible_mul :
+  ∀ a b : Q, rngl_inversible (a * b)%F → rngl_inversible a ∧ rngl_inversible b.
+Proof.
+cbn; unfold Q_inversible.
+intros * Hab.
+apply Decidable.not_or.
+intros H.
+destruct H as [H| H]; [ subst a | subst b ]. {
+  now rewrite Q.mul_0_l in Hab.
+} {
+  now rewrite Q.mul_0_r in Hab.
+}
+Qed.
+
 Theorem Q_consistent :
   rngl_has_inv = false ∨ rngl_has_no_inv_but_div = false.
 Proof. now right. Qed.
@@ -90,6 +107,7 @@ Definition Q_ring_like_prop :=
      rngl_mul_assoc := Q.mul_assoc;
      rngl_mul_1_l := Q.mul_1_l;
      rngl_mul_add_distr_l := Q.mul_add_distr_l;
+     rngl_inversible_mul := Q_inversible_mul;
      rngl_opt_1_neq_0 := Q_1_neq_0;
      rngl_opt_mul_comm := Q.mul_comm;
      rngl_opt_mul_1_r := NA;
