Zrl.v
@@ -8,6 +8,8 @@ Notation "x ≤ y" := (x <= y)%Z (at level 70, y at next level) : Z_scope.
 Notation "x ≤ y ≤ z" := (x <= y ∧ y <= z)%Z (at level 70, y at next level) :
   Z_scope.
 
+Definition Z_inversible x := x ≠ 0%Z.
+
 Definition phony_Z_sub (x y : Z) := 0%Z.
 Definition phony_Z_inv (x : Z) := 0%Z.
 
@@ -22,13 +24,21 @@ Canonical Structure Z_ring_like_op : ring_like_op Z :=
      rngl_opp := Z.opp;
      rngl_inv := phony_Z_inv;
      rngl_le := Z.le;
+     rngl_inversible := Z_inversible;
      rngl_opt_sub := phony_Z_sub;
      rngl_opt_div := Z.div |}.
 
 Existing Instance Z_ring_like_op.
 
-Theorem Z_eq_mul_0 :  ∀ n m, (n * m)%Z = 0%Z → n = 0%Z ∨ m = 0%Z.
-Proof. now apply Z.eq_mul_0. Qed.
+Theorem Z_opt_integral : ∀ a b : Z,
+  rngl_inversible a → rngl_inversible b → rngl_inversible (a * b)%F.
+Proof.
+cbn; unfold Z_inversible.
+intros * Ha Hb.
+intros H.
+apply Z.eq_mul_0 in H.
+now destruct H.
+Qed.
 
 Theorem Z_1_neq_0 : (1 ≠ 0)%Z.
 Proof. easy. Qed.
@@ -101,6 +111,7 @@ Definition Z_ring_like_prop : ring_like_prop Z :=
      rngl_mul_assoc := Z.mul_assoc;
      rngl_mul_1_l := Z.mul_1_l;
      rngl_mul_add_distr_l := Z.mul_add_distr_l;
+     rngl_inversible_mul := Z_inversible_mul;
      rngl_opt_1_neq_0 := Z_1_neq_0;
      rngl_opt_mul_comm := Z.mul_comm;
      rngl_opt_mul_1_r := NA;
@@ -115,7 +126,7 @@ Definition Z_ring_like_prop : ring_like_prop Z :=
      rngl_opt_mul_div_r := NA;
      rngl_opt_eq_dec := Z.eq_dec;
      rngl_opt_le_dec := Z_le_dec;
-     rngl_opt_integral := Z_eq_mul_0;
+     rngl_opt_integral := Z_opt_integral;
      rngl_characteristic_prop := Z_characteristic_prop;
      rngl_opt_le_refl := Z.le_refl;
      rngl_opt_le_antisymm := Z.le_antisymm;
